[DSL] Add a tactic for assembling/splitting invariants

Veil/TransitionSystem.lean
@@ -29,4 +29,47 @@ def invConsecution [RelationalTransitionSystem σ] :=
 def invInductive [sys: RelationalTransitionSystem σ] :=
   @invInit σ sys ∧ @invConsecution σ sys
 
+/-- `invInductive` with the property not necessarily being `inv`. -/
+def isInductiveInvariant [sys: RelationalTransitionSystem σ] (p : σ → Prop) :=
+  (∀ (s : σ), assumptions s → init s → p s) ∧
+  (∀ (s s' : σ), assumptions s → p s → next s s' → p s')
+
+inductive reachable [sys : RelationalTransitionSystem σ] : σ → Prop where
+  | init : ∀ (s : σ), sys.init s → reachable s
+  | step : ∀ (s s' : σ), reachable s → sys.next s s' → reachable s'
+
+theorem reachable_inclusion (sys sys' : RelationalTransitionSystem σ)
+  (hinit_implies : ∀ (st : σ), sys.init st → sys'.init st)
+  (hnext_implies : ∀ (st st' : σ), sys.next st st' → sys'.next st st') :
+  ∀ (st : σ), reachable (sys := sys) st → reachable (sys := sys') st := by
+  intro st h
+  induction h with
+  | init s hinit => apply reachable.init ; apply hinit_implies ; assumption
+  | step s s' h2 hn ih => apply reachable.step ; apply ih ; apply hnext_implies ; assumption
+
+-- another characterization of invariant
+def isInvariant [sys : RelationalTransitionSystem σ] (p : σ → Prop) : Prop := ∀ (s : σ), reachable s → p s
+
+-- theorem invariant_split [sys : RelationalTransitionSystem σ] (p q : σ → Prop) :
+--   (isInvariant (fun s => p s ∧ q s)) = (isInvariant p ∧ isInvariant q) := by
+--   ext ; unfold isInvariant ; simp ; constructor
+--   next => intro h ; constructor <;> intro s hh <;> specialize h s hh <;> cases h <;> assumption
+--   next => intro ⟨ha, hb⟩ s hh ; specialize ha _ hh ; specialize hb _ hh ; constructor <;> assumption
+
+theorem invariant_merge [sys : RelationalTransitionSystem σ] (p q : σ → Prop) :
+  (isInvariant p ∧ isInvariant q) ↔ (isInvariant (fun s => p s ∧ q s)) := by
+  unfold isInvariant ; simp ; constructor
+  next => intro ⟨ha, hb⟩ s hh ; specialize ha _ hh ; specialize hb _ hh ; constructor <;> assumption
+  next => intro h ; constructor <;> intro s hh <;> specialize h s hh <;> cases h <;> assumption
+
+theorem isInductiveInvariant_to_isInvariant [sys : RelationalTransitionSystem σ] (hassu : isInvariant sys.assumptions) (p : σ → Prop) :
+  isInductiveInvariant (sys := sys) p → isInvariant (sys := sys) p := by
+  intro ⟨ha, hb⟩ s h
+  induction h with
+  | init s hinit => specialize hassu _ (.init _ hinit) ; apply ha <;> assumption
+  | step s s' h2 hn ih => specialize hassu _ h2 ; apply hb <;> assumption
+
+theorem invInductive_to_isInvariant [sys : RelationalTransitionSystem σ] (hassu : isInvariant sys.assumptions) :
+  invInductive (sys := sys) → isInvariant (sys := sys) sys.inv := isInductiveInvariant_to_isInvariant hassu sys.inv
+
 end RelationalTransitionSystem
